examples/bytestring/specs.v
@@ -33,6 +33,90 @@ MetaCoq Run (desc_gen EmptyString).
 MetaCoq Run (desc_gen String).
 MetaCoq Run (desc_gen Ascii).
 
+Definition string_get_desc (x : string) : ctor_desc := 
+match x with 
+| EmptyString => (@desc _ EmptyString _)
+| String _ _ =>  (@desc _ String _)
+end.
+  
+Inductive string_has_tag_prop : string -> ctor_desc -> Prop := 
+| tagEmpty : string_has_tag_prop EmptyString (@desc _ EmptyString _)
+| tagString c r : string_has_tag_prop (String c r) (@desc _ String _).
+     
+Definition tag_spec_string : ident * funspec := 
+DECLARE _get_Coq_Strings_String_string_tag
+WITH gv : globals, g : graph, p : rep_type,
+x : string, roots : roots_t, sh : share,
+ti : val, outlier : outlier_t, t_info : GCGraph.thread_info
+PRE  [[  [int_or_ptr_type]  ]]
+PROP (
+  @is_in_graph string _ g x p;
+  writable_share sh  )
+(PARAMSx (  [rep_type_val g p] )
+(GLOBALSx [gv]
+(SEPx (full_gc g t_info roots outlier ti sh gv :: nil))))
+POST [ tuint ]
+(* EX  (xs : args (ctor_reific (nat_get_desc x))), *)
+PROP ( (* 1. x has tag t and is constructed with the constructor description c. 
+              a. Tag function relating to x.
+              b. x = ctor_real c xs (* Doesn't type as this. *)
+
+          TODO: Discuss - something around this should already exist for 
+          generating general in_graph functions, and we want things to match.   
+      *)
+      (* let c := nat_get_desc x in 
+      nat_has_tag_prop x c; *)
+      (* let c := nat_get_desc x in 
+      let r := result (ctor_reific c) xs in
+      @is_in_graph (projT1 r) (@in_graph (projT1 r) (projT2 r)) g (ctor_real c xs) p   *)
+      let c := string_get_desc x in 
+      string_has_tag_prop x c (* Not 100% sure this is how we want it*)
+    )
+RETURN  ( Vint (Int.repr (Z.of_nat (ctor_tag (string_get_desc x)))) )
+SEP (full_gc g t_info roots outlier ti sh gv).
+
+
+
+Definition args_spec_String : funspec := 
+  WITH gv : globals, g : graph, p : rep_type,
+  chs: ascii*string, roots : roots_t, sh : share,
+  ti : val, outlier : outlier_t, t_info : GCGraph.thread_info
+  PRE  [[  [int_or_ptr_type] ]]
+  PROP (
+      writable_share sh;
+          is_in_graph g (String (fst chs) (snd chs)) p  
+      )
+  (PARAMSx ( [rep_type_val g p])
+  (GLOBALSx [gv]
+  (SEPx (full_gc g t_info roots outlier ti sh gv :: nil))))
+  POST [ tptr int_or_ptr_type (* tarray int_or_ptr_type 1 *)  ]
+  EX  (p0 : rep_type) (p1: rep_type) (sh' : share),
+  PROP (  writable_share sh';
+          is_in_graph g (fst chs) p0; is_in_graph g (snd chs) p1
+      )
+  RETURN  ( rep_type_val g p ) 
+  SEP (data_at sh' (tarray int_or_ptr_type 2) [rep_type_val g p0; rep_type_val g p1] (rep_type_val g p);
+      data_at sh' (tarray int_or_ptr_type 2) [rep_type_val g p0; rep_type_val g p1] (rep_type_val g p) -* full_gc g t_info roots outlier ti sh gv). 
+  
+
+Definition ascii_to_char_spec: ident * funspec :=
+ DECLARE _ascii_to_char
+ WITH gv: globals, g: graph, p: rep_type, ch: ascii, roots: roots_t, 
+      sh: share, ti: val, outlier: outlier_t, t_info: GCGraph.thread_info
+ PRE [ int_or_ptr_type ]
+   PROP (readable_share sh; is_in_graph g ch p)
+   PARAMS (rep_type_val g p) GLOBALS (gv)
+   SEP (full_gc g t_info roots outlier ti sh gv)
+ POST [ tuchar ]
+   PROP()
+   RETURN ( Vint (Int.repr (Z.of_N (N_of_ascii ch))) )
+   SEP (full_gc g t_info roots outlier ti sh gv).
+
+
+Definition args_make_Coq_Init_Datatypes_String_String_spec : ident * funspec :=
+DECLARE _get_args
+        (args_spec_String).
+
 Definition make_Coq_Strings_String_string_EmptyString_spec : ident * funspec :=
     DECLARE _make_Coq_Strings_String_string_EmptyString
           (alloc_make_spec_general (@desc _ EmptyString _) 0). 
@@ -57,7 +141,10 @@ Definition append_spec : ident * funspec :=
 
 
 Definition Vprog : varspecs. mk_varspecs prog. Defined.
-Definition Gprog := [ make_Coq_Strings_String_string_EmptyString_spec;
+Definition Gprog := [ ascii_to_char_spec;
+                      tag_spec_string;
+                      args_make_Coq_Init_Datatypes_String_String_spec;
+                      make_Coq_Strings_String_string_EmptyString_spec;
                       alloc_make_Coq_Strings_String_string_String_spec;
                       alloc_make_Coq_Strings_Ascii_ascii_Ascii_spec;
                       gc_spec.garbage_collect_spec
